Minor let_ changes: relabel, re-order length

src/typing/defs.lean
@@ -23,9 +23,9 @@ inductive typing : env V → exp V → typ V → Prop
     , t₁.lc
     → (∀ {x : V}, x ∉ L → typing (insert ⟨x, ⟨0, t₁⟩⟩ Γ) (eb.open_var x) t₂)
     → typing Γ (lam eb) (arr t₁ t₂)
-  | let_ : Π {L₁ L₂ : finset V} {Γ : env V} {ed eb : exp V} {s₁ : sch V} {t₂ : typ V}
-    , (∀ {xs : list V}, s₁.arity = xs.length → xs.nodup → finset.disjoint_list xs L₁ → typing Γ ed (s₁.open_vars xs))
-    → (∀ {x : V}, x ∉ L₂ → typing (insert ⟨x, s₁⟩ Γ) (eb.open_var x) t₂)
-    → typing Γ (let_ ed eb) t₂
+  | let_ : Π {Ld Lb : finset V} {Γ : env V} {ed eb : exp V} {sd : sch V} {tb : typ V}
+    , (∀ {xs : list V}, xs.length = sd.arity → xs.nodup → finset.disjoint_list xs Ld → typing Γ ed (sd.open_vars xs))
+    → (∀ {x : V}, x ∉ Lb → typing (insert ⟨x, sd⟩ Γ) (eb.open_var x) tb)
+    → typing Γ (let_ ed eb) tb
 
 end /- namespace -/ tts --------------------------------------------------------
